ArkLib/CommitmentScheme/QueryCacheToSet.lean
@@ -1,0 +1,52 @@
+
+import VCVio
+import ArkLib.Data.Math.Basic
+import ArkLib.CommitmentScheme.Basic
+import Mathlib.Data.Vector.Snoc
+
+/--
+Returns, for a particular oracle's cache, and a particular oracle index `i`,
+the set of all (query, response) pairs that have been made to the oracle `i`.
+-/
+def QueryCache.toSet {ι : Type} {spec : OracleSpec ι} (i : ι) (cache : spec.QueryCache) :
+    Set (spec.domain i × spec.range i) :=
+  { (q, r) : spec.domain i × spec.range i | cache i q = some r }
+
+@[simp]
+lemma QueryCache.toSet_cacheQuery_eq_insert_of_none {ι : Type} {spec : OracleSpec ι}
+    [spec.DecidableEq] [DecidableEq ι]
+    (i : ι) (cache : spec.QueryCache) (q : spec.domain i) (r : spec.range i)
+    (h : cache i q = none) :
+    QueryCache.toSet i (cache.cacheQuery i q r) =
+      QueryCache.toSet i cache ∪ {(q, r)} := by
+  simp only [QueryCache.toSet, OracleSpec.QueryCache.cacheQuery]
+  simp
+  ext ⟨q', r'⟩
+  simp
+  rw [Function.update_apply]
+  split_ifs with h' <;> simp_all
+  exact eq_comm
+
+
+/-- If the QueryCache.toSet are equal, the underlying caches are equal -/
+@[simp]
+theorem QueryCache.toSet_eq_iff {ι : Type} [Subsingleton ι] {spec : OracleSpec ι}
+    (i : ι) (cache1 cache2 : spec.QueryCache) :
+    QueryCache.toSet i cache1 = QueryCache.toSet i cache2 ↔ cache1 = cache2 := by
+  constructor
+  · intro h
+    sorry
+    -- ext i' d r
+    -- unfold QueryCache.toSet at *
+    -- simp at h
+    -- have : i' = i := by
+    --   -- exact?
+    --   apply Subsingleton.elim
+    -- subst this
+    -- have := congr_fun h (d, r)
+    -- simp at this
+    -- convert this using 1
+
+  · intro h_eq
+    subst h_eq
+    rfl
